Prove covering implies currying defn of subagent

cf5Script.sml
@@ -15,7 +15,8 @@ limitations under the License.
 *)
 
 open HolKernel boolLib bossLib Parse dep_rewrite
-  pred_setTheory categoryTheory cf0Theory cf1Theory cf2Theory
+  pairTheory listTheory pred_setTheory categoryTheory
+  cf0Theory cf1Theory cf2Theory cf4Theory
 
 val _ = new_theory"cf5";
 
@@ -71,13 +72,17 @@ Proof
   \\ fs[cfbot_def, cf1_def, mk_cf_def]
 QED
 
-Theorem subagent_cover:
-  c ◁ d -: w ⇔
+Definition covering_subagent_def:
+  covering_subagent w c d ⇔
     c ∈ chu_objects w ∧ d ∈ chu_objects w ∧
     ∀e. e ∈ c.env ⇒
       ∃f m. f ∈ d.env ∧ m :- c → d -: chu w ∧ e = m.map.map_env f
+End
+
+Theorem subagent_cover:
+  c ◁ d -: w ⇔ covering_subagent w c d
 Proof
-  rw[subagent_def]
+  rw[subagent_def, covering_subagent_def]
   \\ Cases_on`c ∈ chu_objects w` \\ simp[]
   \\ Cases_on`d ∈ chu_objects w` \\ simp[]
   \\ imp_res_tac morphisms_to_cfbot
@@ -116,6 +121,183 @@ Proof
   \\ fs[cfbot_def, is_chu_morphism_def, extensional_def]
   \\ fs[cf1_def, mk_cf_def]
   \\ metis_tac[]
+QED
+
+Definition currying_subagent_def:
+  currying_subagent w c d ⇔
+    c ∈ chu_objects w ∧ d ∈ chu_objects w ∧
+    ∃z. z ∈ chu_objects d.agent ∧ c ≃ move d z -: w
+End
+
+Definition finite_cf_def:
+  finite_cf c ⇔ FINITE c.agent ∧ FINITE c.env
+End
+
+Theorem hom_finite[simp]:
+  finite_cf c ∧ finite_cf d ⇒
+  FINITE (chu w | c → d |)
+Proof
+  rw[hom_def, maps_to_in_chu, finite_cf_def]
+  \\ qspec_then`λm. (m.map.map_agent, m.map.map_env)`irule FINITE_INJ
+  \\ qexists_tac`{f | extensional f c.agent ∧ IMAGE f c.agent ⊆ d.agent} ×
+                 {f | extensional f d.env ∧ IMAGE f d.env ⊆ c.env}`
+  \\ reverse conj_tac
+  >- (
+    simp[INJ_DEF]
+    \\ conj_tac
+    >- ( simp[is_chu_morphism_def] \\ simp[PULL_EXISTS, SUBSET_DEF] )
+    \\ simp[chu_morphism_map_component_equality, morphism_component_equality] )
+  \\ irule FINITE_CROSS
+  \\ conj_tac
+  THENL [qspec_then`λf. IMAGE (λx. (x, f x)) c.agent`irule FINITE_INJ
+         \\ qexists_tac`c` \\ qexists_tac`POW (c.agent × d.agent)`,
+         qspec_then`λf. IMAGE (λx. (x, f x)) d.env`irule FINITE_INJ
+         \\ qexists_tac`d` \\ qexists_tac`POW (d.env × c.env)`]
+  \\ simp[]
+  \\ simp[INJ_DEF, IN_POW]
+  \\ simp[SUBSET_DEF, PULL_EXISTS]
+  \\ simp[EXTENSION, PULL_EXISTS, FORALL_PROD]
+  \\ simp[FUN_EQ_THM, extensional_def]
+  \\ metis_tac[]
+QED
+
+Definition encode_morphism_def:
+  encode_morphism m =
+    encode_pair (encode_function m.dom.agent m.map.map_agent,
+                 encode_function m.cod.env m.map.map_env)
+End
+
+Definition decode_morphism_def:
+  decode_morphism c d s =
+    <| dom := c; cod := d; map := <| map_agent := decode_function (FST (decode_pair s));
+                                     map_env := decode_function (SND (decode_pair s)) |> |>
+End
+
+Theorem decode_encode_morphism[simp]:
+  m.dom = c ∧ m.cod = d ∧ FINITE c.agent ∧ FINITE d.env ∧
+  extensional m.map.map_agent c.agent ∧
+  extensional m.map.map_env d.env
+  ⇒
+  decode_morphism c d (encode_morphism m) = m
+Proof
+  rw[morphism_component_equality, decode_morphism_def]
+  \\ rw[chu_morphism_map_component_equality]
+  \\ rw[encode_morphism_def]
+QED
+
+(*
+Definition encode_hom_def:
+  encode_hom w c d = encode_list (MAP encode_morphism (SET_TO_LIST (chu w | c → d |)))
+End
+
+Definition decode_hom_def:
+  decode_hom c d s = set (MAP (decode_morphism c d) (decode_list s))
+End
+
+Theorem decode_encode_hom[simp]:
+  finite_cf c ∧ finite_cf d ⇒
+  decode_hom c d (encode_hom w c d) = chu w | c → d |
+Proof
+  rw[decode_hom_def, EXTENSION, MEM_MAP, encode_hom_def, PULL_EXISTS]
+  \\ rw[EQ_IMP_THM]
+  \\ TRY(qexists_tac`x` \\ simp[])
+  \\ DEP_REWRITE_TAC[decode_encode_morphism]
+  \\ fs[hom_def, maps_to_in_chu, finite_cf_def]
+  \\ fs[is_chu_morphism_def]
+QED
+*)
+
+Theorem covering_implies_currying:
+  finite_cf c ∧ finite_cf d ∧
+  covering_subagent w c d ⇒ currying_subagent w c d
+Proof
+  rw[covering_subagent_def, currying_subagent_def]
+  \\ qexists_tac`mk_cf <| world := d.agent; agent := c.agent;
+                          env := IMAGE encode_morphism (chu w |c → d|);
+                          eval := λa m. (decode_morphism c d m).map.map_agent a |>`
+  \\ conj_asm1_tac
+  >- (
+    simp[chu_objects_def]
+    \\ simp[SUBSET_DEF, image_def, PULL_EXISTS]
+    \\ rw[hom_def]
+    \\ fs[maps_to_in_chu, finite_cf_def, is_chu_morphism_def] )
+  \\ qmatch_assum_abbrev_tac`z ∈ chu_objects d.agent`
+  \\ simp[homotopy_equiv_def]
+  \\ qexists_tac`mk_chu_morphism c (move d z)
+       <| map_agent := I;
+          map_env := λx. (decode_morphism c d (FST (decode_pair x))).map.map_env
+                           (SND (decode_pair x)) |>`
+  \\ qmatch_goalsub_abbrev_tac`f :- c → move d z -: _`
+  \\ qexists_tac`mk_chu_morphism (move d z) c
+       <| map_agent := I;
+          map_env := λe.
+            let p = @p. (FST p).map.map_env (SND p) = e ∧ (FST p) :- c → d -: chu w ∧
+                        (SND p) ∈ d.env
+            in encode_pair (encode_morphism (FST p), SND p) |>`
+  \\ qmatch_goalsub_abbrev_tac`g :- move d z → _ -: _`
+  \\ conj_asm1_tac
+  >- (
+    simp[maps_to_in_chu, Abbr`f`]
+    \\ simp[mk_chu_morphism_def]
+    \\ simp[is_chu_morphism_def, PULL_EXISTS, FORALL_PROD]
+    \\ simp[restrict_def]
+    \\ simp[Abbr`z`, PULL_EXISTS]
+    \\ CONV_TAC(LAND_CONV(RESORT_FORALL_CONV(sort_vars["x"])))
+    \\ CONV_TAC(RAND_CONV(RESORT_FORALL_CONV(sort_vars["x"])))
+    \\ simp[GSYM FORALL_AND_THM]
+    \\ gen_tac
+    \\ Cases_on`x ∈ chu w |c → d|` \\ simp[]
+    \\ simp[mk_cf_def]
+    \\ gen_tac
+    \\ reverse IF_CASES_TAC >- metis_tac[]
+    \\ pop_assum kall_tac
+    \\ DEP_REWRITE_TAC[decode_encode_morphism]
+    \\ fs[hom_def, maps_to_in_chu, is_chu_morphism_def, finite_cf_def] )
+  \\ conj_asm1_tac
+  >- (
+    simp[Once maps_to_in_chu, Abbr`g`]
+    \\ simp[mk_chu_morphism_def]
+    \\ simp[is_chu_morphism_def]
+    \\ simp[restrict_def]
+    \\ qmatch_goalsub_abbrev_tac`a ∧ b ∧ x`
+    \\ `b` by simp[Abbr`b`, Abbr`z`]
+    \\ qunabbrev_tac`b`
+    \\ simp[]
+    \\ simp[Abbr`a`, Abbr`x`]
+    \\ CONV_TAC(RAND_CONV(SWAP_FORALL_CONV))
+    \\ simp[GSYM FORALL_AND_THM]
+    \\ qx_gen_tac`e`
+    \\ Cases_on`e ∈ c.env` \\ simp[]
+    \\ SELECT_ELIM_TAC
+    \\ conj_tac >- ( simp[EXISTS_PROD] \\ metis_tac[] )
+    \\ simp[FORALL_PROD]
+    \\ qx_gen_tac`g`
+    \\ qx_gen_tac`x`
+    \\ strip_tac
+    \\ simp[Abbr`z`]
+    \\ conj_asm1_tac >- (simp[hom_def] \\ metis_tac[])
+    \\ simp[mk_cf_def, move_def]
+    \\ gen_tac \\ strip_tac
+    \\ DEP_REWRITE_TAC[decode_encode_morphism]
+    \\ fs[maps_to_in_chu, is_chu_morphism_def, finite_cf_def]
+    \\ rpt BasicProvers.VAR_EQ_TAC
+    \\ simp[] )
+  \\ imp_res_tac maps_to_comp \\ fs[]
+  \\ conj_tac \\ irule homotopic_id
+  \\ fs[maps_to_in_chu, pre_chu_def]
+  \\ DEP_REWRITE_TAC[compose_in_thm]
+  \\ DEP_REWRITE_TAC[compose_thm]
+  \\ DEP_REWRITE_TAC[chu_comp]
+  \\ fs[composable_in_def, pre_chu_def]
+  \\ simp[Abbr`f`, Abbr`g`, mk_chu_morphism_def]
+  \\ simp[restrict_def, FUN_EQ_THM, Abbr`z`]
+QED
+
+Theorem currying_implies_covering:
+  finite_cf c ∧ finite_cf d ∧
+  currying_subagent w c d ⇒ covering_subagent w c d
+Proof
+  cheat
 QED
 
 val _ = export_theory();
